src/C_strtoimax/VstProof/AbstractSpecLemmas.v
@@ -1,0 +1,74 @@
+Require Import AbstractSpec.
+Require Import VST.floyd.proofauto.
+
+Definition value_until j l := 
+             (value (Z_of_string (sublist 0 j l))). 
+
+Definition ASN1_INTMAX_MAX := Int64.max_unsigned.
+Definition upper_boundary := Z.div ASN1_INTMAX_MAX 10.
+Definition last_digit_max := Zmod ASN1_INTMAX_MAX 10.
+Definition last_digit_max_minus := last_digit_max + 1.
+
+Lemma lt_ub_bounded : forall j ls, value_until j ls < upper_boundary ->
+                bounded (value_until (j + 1) ls) = true.
+Admitted.
+
+
+Lemma value_always_bounded : forall j ls,
+  0 <= j < Zlength ls 
+  bounded (value_until j ls) = true.
+
+Lemma next_value:
+  forall (ls : list byte) (j : Z),
+    0 <= j + 1 <= Zlength ls ->
+    forall i : byte,
+      Znth j ls = i ->
+      ((Byte.signed i >=? 48) && (Byte.signed i <=? 57))%bool = true ->
+      (value_until (j + 1) ls) =
+      (value_until j ls * 10 + (Byte.signed i - 48)).
+Admitted.
+
+Lemma ub_last_digit_error_range : forall j i i0 ls,
+  0 <= j < Zlength ls ->
+  Znth j ls = i0 ->
+  (value_until j ls > upper_boundary \/
+  (value_until j ls = upper_boundary /\
+  last_digit_max < (Byte.signed i0 - 48))) ->
+  (res (Z_of_string (i :: ls))) = ASN_STRTOX_ERROR_RANGE.
+ Admitted.
+
+Lemma ub_last_digit_error_range_index : forall j i i0 ls,
+  0 <= j < Zlength ls ->
+  Znth j ls = i0 ->
+  (value_until j ls > upper_boundary \/
+  (value_until j ls = upper_boundary /\
+  last_digit_max < (Byte.signed i0 - 48))) ->
+  (index (Z_of_string (i :: ls))) = j + 1.
+ Admitted.
+
+
+Lemma extra_data_index : forall j i ls,
+  0 <= j < Zlength ls ->
+  Znth j ls = i ->
+  is_digit i ->
+  (index (Z_of_string ls)) = j.
+ Admitted.
+
+(** Need a tactic to take out arithmetic hypotheses from this:
+
+H5 : typed_true tint
+         (force_val
+            (sem_cmp_pp Clt
+               (Vptr end'_b (Ptrofs.add (Ptrofs.add str_ofs Ptrofs.one) (Ptrofs.repr j)))
+               (Vptr end'_b end'_ofs))) 
+
+typed_false tint
+          (force_val
+             (sem_cmp_pp Clt
+                (Vptr end'_b
+                   (Ptrofs.add (Ptrofs.add (Ptrofs.add str_ofs Ptrofs.one) (Ptrofs.repr j))
+                      (Ptrofs.mul (Ptrofs.repr 1) (Ptrofs.of_ints (Int.repr 1)))))
+                (Vptr end'_b end'_ofs)))
+
+
+**)
